src/proof/controllers/statefulset/distance_zero_implies_match.v
@@ -1,0 +1,24 @@
+From New.proof.controllers.statefulset Require Export distance.
+From New.proof.controllers.statefulset Require Import common.
+
+Section proof.
+Context `{hG: !heapGS Σ} `{!ffi_semantics _ _}.
+Context {sem : go.Semantics}
+  {package_sem : code.controllers.statefulset.statefulset.Assumptions}.
+Collection W := sem + package_sem.
+Context `{!kubernetesModelG Σ}.
+Local Set Default Proof Using "All".
+
+Lemma distance_zero_implies_match γ sts dqs pods pvcs phase :
+  statefulset_owned_resources γ sts dqs pods pvcs phase -∗
+  ⌜ match_distance sts pods pvcs = 0%nat ↔ current_state_matches sts pods pvcs ⌝.
+Proof.
+  iIntros "Hresources". iNamed "Hresources".
+  iPoseProof (own_pod_frags_living with "Hown_pod_frags") as "%Hpods_living".
+  iPureIntro.
+  apply match_distance_zero_matches_of_living_nodup; last exact Hpods_nodup.
+  intros pod Hpod. rewrite Forall_forall in Hpods_living.
+  apply Hpods_living. by rewrite -list_elem_of_In.
+Qed.
+
+End proof.
